CoqOfNoir/base64/simulation.v
@@ -1,0 +1,182 @@
+Require Import CoqOfNoir.CoqOfNoir.
+Require Import CoqOfNoir.proof.CoqOfNoir.
+Require Import CoqOfNoir.simulation.CoqOfNoir.
+Require CoqOfNoir.base64.translation.
+
+Import Run.
+
+Lemma run_eq₅ {State Address : Set} `{State.Trait State Address}
+    (p : Z) (state : State) (self other : U8.t) :
+  {{ p, state |
+    translation.eq₅ [to_value self; to_value other] ⇓
+    Result.Ok (to_value (Eq.eq self other))
+  | state }}.
+Proof.
+  unfold translation.eq₅.
+  destruct self as [self], other as [other]; cbn.
+  destruct (self =? other) eqn:H_eq; cbn.
+  { apply Run.CallPrimitiveIsEqualTrue; [f_equal; lia|].
+    apply Run.Pure.
+  }
+  { apply Run.CallPrimitiveIsEqualFalse. {
+      assert (self <> other) by lia.
+      congruence.
+    }
+    apply Run.Pure.
+  }
+Qed.
+
+Module Base64EncodeBE.
+  (*
+  struct Base64EncodeBE {
+      table: [u8; 64]
+  }
+  *)
+  Record t : Set := {
+    table : Array.t U8.t (U32.Make 64);
+  }.
+
+  Global Instance Impl_ToValue : ToValue.Trait t := {
+    to_value (x : t) :=
+      Value.Tuple [to_value x.(table)];
+  }.
+
+  (*
+  /// Creates a new encoder that uses the standard Base64 Alphabet (base64) specified in RFC 4648 
+  /// (https://datatracker.ietf.org/doc/html/rfc4648#section-4)
+  fn new() -> Self {
+      Base64EncodeBE {
+          // The alphabet values here are standard UTF-8 (and ASCII) byte encodings, so the index
+          // in the table is the 6-bit Base64 value, and the value at that index is the UTF-8 
+          // encoding of that value.
+          table: [
+              65, 66, 67, 68, 69, 70, 71, 72, 73, 74, 75, 76, 77, 78, 79, 80, 81, 82, 83, 84, 85, 86, 87, 88, 89, 90,// 0-25 (A-Z)
+              97, 98, 99, 100, 101, 102, 103, 104, 105, 106, 107, 108, 109, 110, 111, 112, 113, 114, 115, 116, 117, 118, 119, 120, 121, 122,// 26-51 (a-z)
+              48, 49, 50, 51, 52, 53, 54, 55, 56, 57,// 0-9
+              43,// +
+              47// /
+          ]
+      }
+  }
+  *)
+  Definition new : t := {|
+    table := Array.Make (List.map U8.Make [
+      65; 66; 67; 68; 69; 70; 71; 72; 73; 74; 75; 76; 77; 78; 79; 80; 81; 82; 83; 84; 85; 86; 87; 88; 89; 90;
+      97; 98; 99; 100; 101; 102; 103; 104; 105; 106; 107; 108; 109; 110; 111; 112; 113; 114; 115; 116; 117; 118; 119; 120; 121; 122;
+      48; 49; 50; 51; 52; 53; 54; 55; 56; 57;
+      43;
+      47
+    ])
+  |}.
+
+  Lemma run_new₆ {State Address : Set} `{State.Trait State Address}
+      (p : Z) (state : State) :
+    {{ p, state |
+      translation.new₆ [] ⇓
+      Result.Ok (to_value new)
+    | state }}.
+  Proof.
+    unfold translation.new₆, new.
+    eapply Run.Let. {
+      apply Run.Pure.
+    }
+    apply Run.Pure.
+  Qed.
+End Base64EncodeBE.
+
+(*
+/**
+ * @brief Take an array of ASCII values and convert into base64 values
+ **/
+pub fn base64_encode_elements<let InputElements: u32>(input: [u8; InputElements]) -> [u8; InputElements] {
+    // for some reason, if the lookup table is not defined in a struct, access costs are expensive and ROM tables aren't being used :/
+    let mut Base64Encoder = Base64EncodeBE::new();
+
+    let mut result: [u8; InputElements] = [0; InputElements];
+
+    for i in 0..InputElements {
+        result[i] = Base64Encoder.get(input[i] as Field);
+    }
+    result
+}
+*)
+(* Definition base64_encode_elements {InputElements : U32.t} (input : Array.t U8.t InputElements) :
+    Array.t U8.t InputElements :=
+  let Base64Encoder := Base64EncodeBE.new in
+
+  let result : Array.t U8.t InputElements := Array.repeat InputElements (U8.Make 0) in
+
+  M.for_Z (Integer.to_Z InputElements) (fun (i : Z) =>
+    let i : U32.t := U32.Make i in
+    Array.write result i (Base64Encoder.get (U8.to_Z (Array.get input i)))
+  ); result. *)
+
+(* Lemma run_eq₂ {State Address : Set} `{State.Trait State Address}
+    (state : State) (self other : Array.t U8.t 36) :
+  {{ state |
+    translation.eq₂ [to_value self; to_value other] ⇓
+    Result.Ok (to_value (Eq.eq self other))
+  | state }}.
+Proof.
+  unfold translation.eq₂. *)
+
+(*
+pub fn base64_encode<let InputBytes: u32, let OutputElements: u32>(input: [u8; InputBytes]) -> [u8; OutputElements] {
+    // 240 bits fits 40 6-bit chunks and 30 8-bit chunks
+    // we pack 40 base64 values into a field element and convert into 30 bytes
+    // TODO: once we support arithmetic ops on generics, derive OutputBytes from InputBytes
+    let mut result: [u8; OutputElements] = [0; OutputElements];
+    let BASE64_ELEMENTS_PER_CHUNK: u32 = 40;
+    let BYTES_PER_CHUNK: u32 = 30;
+    let num_chunks = (InputBytes / BYTES_PER_CHUNK) + (InputBytes % BYTES_PER_CHUNK != 0) as u32;
+
+    if num_chunks > 0 {
+        for i in 0..num_chunks - 1 {
+            let mut slice: Field = 0;
+            for j in 0..BYTES_PER_CHUNK {
+                slice *= 256;
+                slice += input[i * BYTES_PER_CHUNK + j] as Field;
+            }
+
+            let slice_base64_chunks: [u8; 40] = slice.to_be_radix(64);
+            for j in 0..BASE64_ELEMENTS_PER_CHUNK {
+                result[i * BASE64_ELEMENTS_PER_CHUNK + j] = slice_base64_chunks[j];
+            }
+        }
+
+        let bytes_in_final_chunk = InputBytes - ((num_chunks - 1) * BYTES_PER_CHUNK);
+
+        let mut slice: Field = 0;
+        for j in 0..bytes_in_final_chunk {
+            slice *= 256;
+            slice += input[(num_chunks - 1) * BYTES_PER_CHUNK + j] as Field;
+        }
+        for _ in bytes_in_final_chunk..BYTES_PER_CHUNK {
+            slice *= 256;
+        }
+
+        // TODO: check is it cheaper to use a constant value in `to_be_bytes` or can we use `bytes_in_final_chunk`?
+        let slice_base64_chunks: [u8; 40] = slice.to_be_radix(64);
+
+        let num_elements_in_final_chunk = OutputElements - ((num_chunks - 1) * BASE64_ELEMENTS_PER_CHUNK);
+        for i in 0..num_elements_in_final_chunk {
+            result[(num_chunks - 1) * BASE64_ELEMENTS_PER_CHUNK + i] = slice_base64_chunks[i];
+        }
+        result = base64_encode_elements(result);
+    }
+
+    result
+}
+*)
+(* Definition base64_encode {InputBytes OutputElements : U32.t} (input : Array.t U8.t InputBytes) :
+    Array.t U8.t OutputElements :=
+  let result : Array.t U8.t OutputElements := Array.repeat OutputElements (U8.Make 0) in
+  let BASE64_ELEMENTS_PER_CHUNK : U32.t := U32.Make 40 in
+  let BYTES_PER_CHUNK : U32.t := U32.Make 30 in
+  let num_chunks : U32.t :=
+    Integer.add
+      (Integer.div InputBytes BYTES_PER_CHUNK)
+      (Integer.of_bool (negb (Eq.eq (Integer.mod_ InputBytes BYTES_PER_CHUNK) (U32.Make 0)))) in
+
+  if Integer.to_Z num_chunks >? 0 then
+    M.for_ () *)
